Logic/Modal/Standard/Kripke/Geach/Definability.lean
@@ -8,50 +8,36 @@ namespace LO.Modal.Standard
 open System
 open System.Axioms (Geach)
 
-variable [Inhabited W] [Inhabited α]
+namespace Kripke
 
-def Kripke.GeachConfluent (l : Geach.Taple) : Kripke.FrameProperty α := λ F => ∀ {x y z}, (F^[l.i] x y) ∧ (F^[l.j] x z) → ∃ u, (F^[l.m] y u) ∧ (F^[l.n] z u)
+variable [Inhabited α]
+
+def GeachConfluent (t : Geach.Taple) : FrameProperty := λ F => ∀ {x y z : F.World}, (x ≺^[t.i] y) ∧ (x ≺^[t.j] z) → ∃ u, (y ≺^[t.m] u) ∧ (z ≺^[t.n] u)
 
 @[simp]
-def Kripke.MultiGeachConfluent (l : List Geach.Taple) : Kripke.FrameProperty α :=
-  match l with
+def MultiGeachConfluent (ts : List Geach.Taple) : FrameProperty :=
+  match ts with
   | [] => λ _ => True
-  | x :: xs => λ F => (GeachConfluent x F) ∧ (MultiGeachConfluent xs F)
+  | t :: ts => λ F => (GeachConfluent t F) ∧ (MultiGeachConfluent ts F)
 
-namespace Kripke.GeachConfluent
+namespace GeachConfluent
 
-variable {F : Kripke.Frame W α}
+variable {F : Frame}
 
-@[simp]
-lemma serial_def : (GeachConfluent ⟨0, 0, 1, 1⟩ F) ↔ Serial F := by
-  simp [GeachConfluent, Symmetric];
-  aesop;
+@[simp] lemma serial_def : (GeachConfluent ⟨0, 0, 1, 1⟩ F) ↔ Serial F.Rel := by simp [GeachConfluent, Symmetric]; aesop;
 
-@[simp]
-lemma reflexive_def : (GeachConfluent ⟨0, 0, 1, 0⟩ F) ↔ Reflexive F := by
-  simp [GeachConfluent, Reflexive];
+@[simp] lemma reflexive_def : (GeachConfluent ⟨0, 0, 1, 0⟩ F) ↔ Reflexive F.Rel := by simp [GeachConfluent, Reflexive];
 
-@[simp]
-lemma symmetric_def : (GeachConfluent ⟨0, 1, 0, 1⟩ F) ↔ Symmetric F := by
-  simp [GeachConfluent, Symmetric];
-  aesop;
+@[simp] lemma symmetric_def : (GeachConfluent ⟨0, 1, 0, 1⟩ F) ↔ Symmetric F.Rel := by simp [GeachConfluent, Symmetric]; aesop;
+
+@[simp] lemma transitive_def : (GeachConfluent ⟨0, 2, 1, 0⟩ F) ↔ Transitive F.Rel := by simp [GeachConfluent, Transitive]; aesop;
+
+@[simp] lemma euclidean_def : (GeachConfluent ⟨1, 1, 0, 1⟩ F) ↔ Euclidean F.Rel := by simp [GeachConfluent, Euclidean]; aesop;
+
+@[simp] lemma confluent_def : (GeachConfluent ⟨1, 1, 1, 1⟩ F) ↔ Confluent F.Rel := by simp [GeachConfluent, Confluent];
 
 @[simp]
-lemma transitive_def : (GeachConfluent ⟨0, 2, 1, 0⟩ F) ↔ Transitive F := by
-  simp [GeachConfluent, Transitive];
-  aesop;
-
-@[simp]
-lemma euclidean_def : (GeachConfluent ⟨1, 1, 0, 1⟩ F) ↔ Euclidean F := by
-  simp [GeachConfluent, Euclidean];
-  aesop;
-
-@[simp]
-lemma confluent_def : (GeachConfluent ⟨1, 1, 1, 1⟩ F) ↔ Confluent F := by
-  simp [GeachConfluent, Confluent];
-
-@[simp]
-lemma extensive_def : (GeachConfluent ⟨0, 1, 0, 0⟩ F) ↔ Extensive F := by
+lemma extensive_def : (GeachConfluent ⟨0, 1, 0, 0⟩ F) ↔ Extensive F.Rel := by
   intros;
   simp [GeachConfluent, Extensive];
   constructor;
@@ -64,29 +50,36 @@ lemma extensive_def : (GeachConfluent ⟨0, 1, 0, 0⟩ F) ↔ Extensive F := by
     subst hxy this;
     trivial;
 
-@[simp]
-lemma functional_def : Functional F ↔ (GeachConfluent ⟨1, 1, 0, 0⟩ F) := by
-  simp [GeachConfluent, Functional];
-  aesop
+@[simp] lemma functional_def : (GeachConfluent ⟨1, 1, 0, 0⟩ F) ↔ Functional F.Rel := by simp [GeachConfluent, Functional]; aesop
+
+@[simp] lemma dense_def : (GeachConfluent ⟨0, 1, 2, 0⟩ F)  ↔ Dense F.Rel := by simp [GeachConfluent, Dense]; aesop;
+
+@[simp] def TrivialFrame : FiniteFrame := { World := PUnit, Rel := λ _ _ => True }
 
 @[simp]
-lemma dense_def : Dense F  ↔ (GeachConfluent ⟨0, 1, 2, 0⟩ F) := by
-  simp [GeachConfluent, Dense];
-  aesop;
-
-lemma multiframe_trivial_frame : (@Multiframe PUnit α inferInstance (λ _ _ => True) n x y) ↔ (x = y) := by induction n <;> simp_all;
-
-@[simp]
-lemma trivial_frame : GeachConfluent (W := PUnit) (α := α) t (λ _ _ => True) := by simp [GeachConfluent, multiframe_trivial_frame];
-
-end Kripke.GeachConfluent
-
-namespace Kripke.MultiGeachConfluent
+private lemma trivial_frame_relItr : Frame.RelItr n (F := { World := PUnit, Rel := λ _ _ => True }) x y ↔ x = y := by
+  induction n with
+  | zero => simp;
+  | succ n ih => simp; use PUnit.unit; simp_all;
 
 @[simp]
-lemma trivial_frame : MultiGeachConfluent (W := PUnit) (α := α) l (λ _ _ => True) := by induction l <;> simp [MultiGeachConfluent, *];
+lemma trivial_frame : GeachConfluent t { World := PUnit, Rel := λ _ _ => True } := by simp [GeachConfluent, trivial_frame_relItr.mpr];
 
-end Kripke.MultiGeachConfluent
+end GeachConfluent
+
+
+namespace MultiGeachConfluent
+
+@[simp]
+lemma trivial_frame : MultiGeachConfluent ts { World := PUnit, Rel := λ _ _ => True } := by
+  induction ts with
+  | nil => simp;
+  | cons t ts ih =>
+    constructor;
+    . exact Kripke.GeachConfluent.trivial_frame;
+    . exact ih;
+
+end MultiGeachConfluent
 
 
 open Kripke
@@ -96,57 +89,46 @@ open AxiomSet
 variable {Ax : AxiomSet α}
 
 instance AxiomSet.Geach.definability (t) : Definability (α := α) 𝗴𝗲(t) (GeachConfluent t) where
-  defines W _ F := by
-    simp [AxiomSet.Geach, GeachConfluent, Geach];
+  defines F := by
+    simp [AxiomSet.Geach, GeachConfluent];
     constructor;
     . intro h x y z hi hj;
-      let M : Model W α := {
-        frame := F,
-        valuation := λ v _ => F^[t.m] y v
-      }
-      have him : (M, x) ⊧ ◇^[t.i](□^[t.m](Formula.atom default)) := by
+      let M : Model α := { Frame := F, Valuation := λ v _ => y ≺^[t.m] v }
+      have him_x : Satisfies M x (◇^[t.i](□^[t.m](Formula.atom default))) := by
         apply Satisfies.multidia_def.mpr;
         existsi y;
         constructor;
         . simpa;
         . apply Satisfies.multibox_def.mpr; aesop;
-      have : (M, x) ⊧ □^[t.j](◇^[t.n]atom default) := (Semantics.Tarski.realize_imp.mp (h (Formula.atom default) M.valuation x)) him;
-      have : (M, z) ⊧ ◇^[t.n]atom default := Satisfies.multibox_def.mp this z hj;
-      obtain ⟨u, hzu, hyu⟩ := Satisfies.multidia_def.mp this;
+      have hjn_x : Satisfies M x (□^[t.j](◇^[t.n]atom default)) := Kripke.Satisfies.mdp (h (Formula.atom default) M.Valuation x) him_x;
+      have hn_z : Satisfies M z (◇^[t.n]atom default) := Satisfies.multibox_def.mp hjn_x z hj;
+      obtain ⟨u, hzu, hyu⟩ := Satisfies.multidia_def.mp hn_z;
       existsi u;
       exact ⟨hyu, hzu⟩;
-    . intro h p V w;
-      simp only [Semantics.Tarski.realize_imp, Satisfies.multibox_def];
-      intro him;
-      obtain ⟨y, hy, hpy⟩ := Satisfies.multidia_def.mp him;
-      intro z hxz;
-      obtain ⟨u, hyu, hzu⟩ := h hy hxz;
-      apply Satisfies.multidia_def.mpr;
-      existsi u;
+    . intro h p V x;
+      simp [AxiomSet.Geach];
+      intro y hxy hm z hxz;
+      obtain ⟨u, hyu, hzu⟩ := h hxy hxz;
+      use u;
       constructor;
       . assumption;
-      . exact Satisfies.multibox_def.mp hpy u hyu;
+      . exact hm u hyu;
 
-instance AxiomSet.IsGeach.definability [Ax.IsGeach] : Definability Ax (Kripke.GeachConfluent (IsGeach.taple Ax)) where
-  defines W _ F := by convert (AxiomSet.Geach.definability _ |>.defines W F); exact IsGeach.char;
-
-instance AxiomSet.MultiGeach.definability (l) : Definability (α := α) 𝗚𝗲(l) (Kripke.MultiGeachConfluent l) where
-  defines W _ F := by
-    induction l with
+instance AxiomSet.MultiGeach.definability (ts) : Definability (α := α) 𝗚𝗲(ts) (Kripke.MultiGeachConfluent ts) where
+  defines F := by
+    induction ts with
     | nil => apply AxiomSet.K.definability.defines;
     | cons t ts ih =>
       simp only [MultiGeach.iff_cons, Semantics.RealizeSet.union_iff, MultiGeachConfluent];
       constructor;
       . rintro ⟨ht, hts⟩;
         constructor;
-        . exact AxiomSet.Geach.definability t |>.defines W F |>.mp ht;
+        . exact AxiomSet.Geach.definability t |>.defines F |>.mp ht;
         . apply ih.mp hts;
       . rintro ⟨ht, hts⟩;
         constructor;
-        . exact AxiomSet.Geach.definability t |>.defines W F |>.mpr ht;
+        . exact AxiomSet.Geach.definability t |>.defines F |>.mpr ht;
         . apply ih.mpr hts;
-
-namespace Kripke
 
 variable {L : DeductionParameter α} [L.HasNec]
 
@@ -154,20 +136,16 @@ instance instGeachDefinability [geach : L.IsGeach] : Definability Ax(L) (Kripke.
   convert AxiomSet.MultiGeach.definability (α := α) geach.taples;
   simp;
 
-instance : FiniteFrameClass.Nonempty (α := α) 𝔽(𝗚𝗲(l))ꟳ where
-  W := PUnit;
-  W_inhabited := inferInstance;
-  W_finite := inferInstance;
-  existsi := by
-    existsi (λ _ _ => True);
-    apply iff_definability_memAxiomSetFrameClass (AxiomSet.MultiGeach.definability l) |>.mpr;
-    simp only [MultiGeachConfluent.trivial_frame];
+instance : FiniteFrameClass.IsNonempty (𝔽ꟳ(𝗚𝗲(l)) : FiniteFrameClass' α) := by
+  existsi { World := PUnit, Rel := λ _ _ => True };
+  apply iff_definability_memAxiomSetFrameClass (AxiomSet.MultiGeach.definability l) |>.mpr;
+  exact MultiGeachConfluent.trivial_frame;
 
-instance : FrameClass.Nonempty (α := α) 𝔽(𝗚𝗲(l)) := inferInstance
+instance : FrameClass.IsNonempty (𝔽(𝗚𝗲(l)) : FrameClass' α) := inferInstance
 
 instance : System.Consistent (𝐆𝐞(l) : DeductionParameter α) := inferInstance
 
-instance [geach : L.IsGeach] : FrameClass.Nonempty 𝔽(Ax(L)) := by rw [geach.char]; infer_instance
+instance [geach : L.IsGeach] : FrameClass.IsNonempty 𝔽(Ax(L)) := by rw [geach.char]; infer_instance;
 
 instance [L.IsGeach] : System.Consistent L := inferInstance
 
@@ -175,13 +153,9 @@ instance : System.Consistent (𝐒𝟒 : DeductionParameter α) := inferInstance
 
 instance : System.Consistent (𝐒𝟓 : DeductionParameter α) := inferInstance
 
-instance : Definability (α := α) Ax(𝐒𝟒) (λ F => Reflexive F ∧ Transitive F) := by simpa using instGeachDefinability (L := 𝐒𝟒)
+instance : Definability (α := α) Ax(𝐒𝟒) (λ F => Reflexive F.Rel ∧ Transitive F.Rel) := by simpa using instGeachDefinability (L := 𝐒𝟒)
 
-/-
-
-instance AxiomSet.S5.definability : Definability (α := α) 𝐒𝟓 (λ F => Reflexive F ∧ Euclidean F) := by
-  simpa using AxiomSet.IsGeachLogic.definability (Ax := 𝐒𝟓);
--/
+instance : Definability (α := α) Ax(𝐒𝟓) (λ F => Reflexive F.Rel ∧ Euclidean F.Rel) := by simpa using instGeachDefinability (L := 𝐒𝟓);
 
 end Kripke
 
