Logic/Modal/Standard/Kripke/Reducible.lean
@@ -8,34 +8,34 @@ namespace Kripke
 variable
   {α : Type u} [DecidableEq α]
   {L₁ L₂ : DeductionParameter α} [L₁.HasNec] [L₂.HasNec]
-  {P₁ P₂ : FrameProperty α}
+  {P₁ P₂ : FrameProperty}
   [sound₁ : Sound L₁ 𝔽(Ax(L₁))] [sound₂ : Sound L₂ 𝔽(Ax(L₂))]
   [complete₁ : Complete L₁ 𝔽(Ax(L₁))] [complete₂ : Complete L₂ 𝔽(Ax(L₂))]
   [definability₁ : Definability Ax(L₁) P₁] [definability₂ : Definability Ax(L₂) P₂]
 
-lemma reducible_of_subset_axiomSetFrameClass (hs : ∀ {W}, [Inhabited W] → ∀ {F}, 𝔽(Ax(L₂)) W F → 𝔽(Ax(L₁)) W F) : L₁ ≤ₛ L₂ := by
+lemma reducible_of_subset_axiomSetFrameClass (hs : ∀ {F}, F ∈ 𝔽(Ax(L₂)) → F ∈ 𝔽(Ax(L₁))) : L₁ ≤ₛ L₂ := by
   apply System.reducible_iff.mpr;
   intro p hp;
   apply complete₂.complete;
-  intro W _ F hF;
-  exact sound₁.sound hp W F $ hs hF;
+  intro F hF;
+  exact sound₁.sound hp F $ hs hF;
 
-lemma reducible_of_definability (hs : ∀ {W}, [Inhabited W] → ∀ {F : Frame W α}, P₂ F → P₁ F) : L₁ ≤ₛ L₂ := by
+lemma reducible_of_definability (hs : ∀ {F : Frame}, P₂ F → P₁ F) : L₁ ≤ₛ L₂ := by
   apply reducible_of_subset_axiomSetFrameClass;
-  intro W _ F hF;
+  intro F hF;
   apply iff_definability_memAxiomSetFrameClass definability₁ |>.mpr;
   exact hs $ iff_definability_memAxiomSetFrameClass definability₂ |>.mp hF;
 
 lemma equiv_of_eq_axiomSetFrameClass
-  (hs₁ : ∀ {W}, [Inhabited W] → ∀ {F}, 𝔽(Ax(L₂)) W F → 𝔽(Ax(L₁)) W F)
-  (hs₂ : ∀ {W}, [Inhabited W] → ∀ {F}, 𝔽(Ax(L₁)) W F → 𝔽(Ax(L₂)) W F)
+  (hs₁ : ∀ {F}, F ∈ 𝔽(Ax(L₂)) → F ∈ 𝔽(Ax(L₁)))
+  (hs₂ : ∀ {F}, F ∈ 𝔽(Ax(L₁)) → F ∈ 𝔽(Ax(L₂)))
   : L₁ =ₛ L₂ := by
   apply System.Equiv.antisymm_iff.mpr;
   constructor;
   . apply reducible_of_subset_axiomSetFrameClass hs₁;
   . apply reducible_of_subset_axiomSetFrameClass hs₂;
 
-lemma equiv_of_iff_definability (h : ∀ {W}, [Inhabited W] → ∀ {F : Frame W α}, P₁ F ↔ P₂ F) : L₁ =ₛ L₂ := by
+lemma equiv_of_iff_definability (h : ∀ {F}, P₁ F ↔ P₂ F) : L₁ =ₛ L₂ := by
   apply System.Equiv.antisymm_iff.mpr;
   constructor;
   . apply reducible_of_definability (definability₁ := definability₁) (definability₂ := definability₂); intros; exact h.mpr (by assumption)
